---
title: Roots of a Quadratic Equation  
subtitle: IITM Quiz 1
description: If $ \alpha $ and $ \beta $ are the roots of $ x^2 + 4x + 1 = 0 $, then the equation whose roots are $ \alpha^2 $ and $ \beta^2 $ is?
weight: 1
categories:
- Quadratic Equation
---

---





### 3Ô∏è‚É£ Roots of a Quadratic Equation

**Question:**
If \$ \alpha \$ and \$ \beta \$ are the roots of \$ x^2 + 4x + 1 = 0 \$, then the equation whose roots are \$ \alpha^2 \$ and \$ \beta^2 \$ is:


## Step-by-Step Solution with Formulas ‚ú®

Let's find the quadratic equation whose roots are \$ \alpha^2 \$ and \$ \beta^2 \$, given that \$ \alpha \$ and \$ \beta \$ are the roots of \$ x^2 + 4x + 1 = 0 \$.

### 1. **Identify the Sums and Products of the Original Roots**

For a quadratic equation \$ x^2 + px + q = 0 \$:

- **Sum of roots:** \$ \alpha + \beta = -p \$
- **Product of roots:** \$ \alpha \beta = q \$

So, for \$ x^2 + 4x + 1 = 0 \$:

- \$ \alpha + \beta = -4 \$
- \$ \alpha \beta = 1 \$


### 2. **Find the Sum of the Squares of the Roots**

Use the formula:

$$
\alpha^2 + \beta^2 = (\alpha + \beta)^2 - 2\alpha\beta
$$

Plug in the values:

$$
\alpha^2 + \beta^2 = (-4)^2 - 2 \times 1 = 16 - 2 = 14
$$

### 3. **Find the Product of the Squares of the Roots**

Use the formula:

$$
\alpha^2 \beta^2 = (\alpha \beta)^2
$$

Plug in the value:

$$
\alpha^2 \beta^2 = (1)^2 = 1
$$

### 4. **Form the New Quadratic Equation**

A quadratic equation with roots \$ r_1 \$ and \$ r_2 \$ is:

$$
x^2 - (r_1 + r_2)x + (r_1 r_2) = 0
$$

So, for roots \$ \alpha^2 \$ and \$ \beta^2 \$:

$$
x^2 - (\alpha^2 + \beta^2)x + (\alpha^2 \beta^2) = 0
$$

Substitute the calculated values:

$$
x^2 - 14x + 1 = 0
$$

### 5. **Final Answer**

> The required quadratic equation whose roots are \$ \alpha^2 \$ and \$ \beta^2 \$ is:
>

> $$
> \boxed{x^2 - 14x + 1 = 0}
>
$$

### **Summary Table**

| Step | Formula Used | Value |
| :-- | :-- | :-- |
| Sum of roots | \$ \alpha + \beta = -p \$ | \$ -4 \$ |
| Product of roots | \$ \alpha \beta = q \$ | \$ 1 \$ |
| Sum of squares | \$ (\alpha + \beta)^2 - 2\alpha\beta \$ | \$ 14 \$ |
| Product of squares | \$ (\alpha\beta)^2 \$ | \$ 1 \$ |
| New equation | \$ x^2 - (sum)x + (product) = 0 \$ | \$ x^2 - 14x + 1 = 0 \$ |

**That‚Äôs how you find the new quadratic equation step by step, using formulas at every stage! üöÄ**

---

### How to Find the Sum and Product of Roots in a Quadratic Equation üßÆ

Let's break down how the sum and product of roots are found for a quadratic equation like
\$ x^2 + 4x + 1 = 0 \$.

### 1. **General Formula for a Quadratic Equation**

A quadratic equation is usually written as:

$$
ax^2 + bx + c = 0
$$

- The roots (solutions) are usually called \$ \alpha \$ and \$ \beta \$.


### 2. **Formulas for Sum and Product of Roots**

For the equation \$ ax^2 + bx + c = 0 \$:

- **Sum of roots:**

$$
\alpha + \beta = -\frac{b}{a}
$$
- **Product of roots:**

$$
\alpha \beta = \frac{c}{a}
$$


### 3. **Apply to the Given Equation**

Given:
\$ x^2 + 4x + 1 = 0 \$

- Here, \$ a = 1 \$, \$ b = 4 \$, \$ c = 1 \$

So:

- **Sum of roots:**

$$
\alpha + \beta = -\frac{4}{1} = -4
$$
- **Product of roots:**

$$
\alpha \beta = \frac{1}{1} = 1
$$


### 4. **Summary Table**

| Formula | Calculation | Result |
| :-- | :-- | :-- |
| \$ \alpha + \beta = -\frac{b}{a} \$ | \$ -\frac{4}{1} \$ | \$ -4 \$ |
| \$ \alpha \beta = \frac{c}{a} \$ | \$ \frac{1}{1} \$ | \$ 1 \$ |

### 5. **Emoji Recap!**

- ‚úçÔ∏è **Sum of roots:** Just take the negative of the coefficient of \$ x \$ and divide by the coefficient of \$ x^2 \$!
- ‚úçÔ∏è **Product of roots:** Just divide the constant term by the coefficient of \$ x^2 \$!

**That's how the sum and product of roots are found for any quadratic equation!** üöÄ

