---
title: Activity Questions 2.6
date: 2025-05-08
tags:
  - Notes 
  - IIT Madras
excludeSearch: false
weight: 26.5
---


{{< border >}}
## Multiple Choice Questions (MCQ):

**Question 1:** If a line is perpendicular to the X-axis, then the slope of such line is _______

Options:

- 0
- Not defined
- 1
- -1
{{< /border >}}

{{< border type="tip" title="Solution" >}}

{{< /border >}}


{{< border >}}
**Question 2:** If a line is parallel to a line which is perpendicular to the Y-axis, then the slope of the first line is _______

Options:

- 0
- Not defined
- 1
- -1
{{< /border >}}

{{< border type="tip" title="Solution" >}}

{{< /border >}}


{{< border >}}
**Question 3:** The angle formed by the intersection of 2 lines with slopes 1 and -1 is _______

Options:

- 0 degree
- 45 degree
- 90 degree
- 180 degree
{{< /border >}}

{{< border type="tip" title="Solution" >}}

{{< /border >}}


{{< border >}}
## Multiple Select Questions (MSQ):

**Question 4:** If l₁ and l₂ are lines parallel to each other with slopes m₁ and m₂ and with inclinations α and β respectively, then which of the following is/are correct?

Options:

- α = β and, tan α = tan β
- α ≠ β and, tan α ≠ tan β
- m₁ = m₂, always
- m₁ × m₂ = -1
{{< /border >}}

{{< border type="tip" title="Solution" >}}

{{< /border >}}


{{< border >}}
**Question 5:** Lines l₁ and l₂ are perpendicular to each other with slopes m₁ and m₂ and with inclinations α and β respectively. Then, which of the following is/are correct?

Options:

- α = β and, tan α = tan β
- β = 90 + α, and tan α = -cot β
- β = 90 + α, and tan β = -cot α
- m₂ = -1/m₁
{{< /border >}}

{{< border type="tip" title="Solution" >}}

{{< /border >}}


{{< border >}}
**Question 6:** If two lines l₁ and l₂ with slopes m₁ and m₂ and inclinations α₁ and α₂ (α₂ > α₁) respectively intersect each other and make an acute angle θ and an obtuse angle φ, then which of the following is/are correct?

**Note:** θ = (α₂ - α₁)

Options:

- tan θ = (tan α₂ - tan α₁)/(1 + tan α₁ × tan α₂) ≠ (m₁ - m₂)/(1 + m₁ × m₂)
- m₁ × m₂ = (-1)
- tan φ = (m₁ - m₂)/(1 + m₁ × m₂)
- tan θ = tan (α₂ - α₁)
{{< /border >}}

{{< border type="tip" title="Solution" >}}

{{< /border >}}


{{< border >}}

{{< /border >}}

{{< border type="tip" title="Solution" >}}

{{< /border >}}


{{< border >}}

{{< /border >}}

{{< border type="tip" title="Solution" >}}

{{< /border >}}


